bootstrap/compileCallReplStepDecScript.sml
@@ -8,7 +8,7 @@ val bootstrap_lcode_def = new_definition("bootstrap_lcode_def",
         rand(rand(rator(rand(rand(rand(rand(rhs(concl(repl_decs_compiled)))))))))))
 
 val rev_bootstrap_lcode = save_thm("rev_bootstrap_lcode",
-  (RAND_CONV(REWR_CONV bootstrap_lcode_def) THENC EVAL) ``REVERSE bootstrap_lcode``)
+  (RAND_CONV(REWR_CONV bootstrap_lcode_def) THENC listLib.REVERSE_CONV) ``REVERSE bootstrap_lcode``)
 
 val internal_contab_def = new_definition("internal_contab_def",
   mk_eq(``internal_contab:contab``, rand(rator(rhs(concl(repl_decs_compiled))))))
@@ -17,15 +17,14 @@ val compile_repl_decs_internal =
   CONV_RULE(LAND_CONV(REWRITE_CONV[SYM compile_repl_decs_def]))
     (REWRITE_RULE[SYM bootstrap_lcode_def, SYM internal_contab_def]repl_decs_compiled)
 
-val _ = computeLib.add_funs[call_repl_step_dec_def,compile_repl_decs_internal]
+val _ = computeLib.add_funs[compile_repl_decs_internal]
 
 val call_repl_step_dec_compiled = save_thm("call_repl_step_dec_compiled",
   EVAL``
-    let m = FST(SND(compile_repl_decs)) in
     let env = FST(SND(SND(compile_repl_decs))) in
     let rsz = FST(SND(SND(SND(compile_repl_decs)))) in
     let cs = SND(SND(SND(SND(compile_repl_decs)))) in
-  compile_dec FEMPTY m env rsz <|out:=[];next_label:=cs.next_label|> call_repl_step_dec``);
+  compile FEMPTY env TCNonTail rsz <|out:=[];next_label:=cs.next_label|> (CCall T (CVar(Short 0)) [CLit Unit])``);
 
 val code_labels_ok_rev_bootstrap_lcode =
   ASSUME ``code_labels_ok (REVERSE bootstrap_lcode)``
@@ -37,12 +36,10 @@ val code_labels_rev_bootstrap_lcode = save_thm("code_labels_rev_bootstrap_lcode"
     ``code_labels real_inst_length (REVERSE bootstrap_lcode)``)
 
 val call_lcode_def = new_definition("call_lcode_def",
-  mk_eq(``call_lcode:bc_inst list``,rand(rand(rator(rand(rhs(concl(call_repl_step_dec_compiled))))))))
-
-val gen_fmap_defs = (map (fst o snd) o DB.find)"gen_fmap_"
+  mk_eq(``call_lcode:bc_inst list``,rand(rand(rator(rhs(concl(call_repl_step_dec_compiled)))))))
 
 val rev_call_lcode = save_thm("rev_call_lcode",
-  (RAND_CONV(REWR_CONV call_lcode_def) THENC REWRITE_CONV(gen_fmap_defs) THENC EVAL) ``REVERSE call_lcode``)
+  (RAND_CONV(REWR_CONV call_lcode_def) THENC listLib.REVERSE_CONV) ``REVERSE call_lcode``)
 
 val code_labels_ok_rev_call_lcode =
   ASSUME ``code_labels_ok (REVERSE call_lcode)``
